[llir-semantics] Progress on closures

Maps.v
@@ -10,6 +10,7 @@ Require Import Coq.Classes.EquivDec.
 
 Import ListNotations.
 
+Set Implicit Arguments.
 
 Module Type PARTIAL_MAP.
   Parameter key: Type.
@@ -74,35 +75,86 @@ Module PTrie <: PARTIAL_MAP.
 
   Definition empty (V: Type) := Leaf : tree V.
 
-  Fixpoint get (V: Type) (a: t V) (key: positive): option V :=
-    match a with
-    | Leaf => None
-    | Node l o r =>
-        match key with
-        | xH => o
-        | xO ii => get V l ii
-        | xI ii => get V r ii
-        end
-    end.
+  Arguments empty {V}.
 
-  Fixpoint set (V: Type) (a: t V) (key: positive) (v: V): t V :=
-    match key with
-    | xH =>
+  Section GET.
+    Variable V: Type.
+
+    Fixpoint get (a: t V) (key: positive): option V :=
       match a with
-      | Leaf => Node Leaf (Some v) Leaf
-      | Node l _ r => Node l (Some v) r
-      end
-    | xO ii =>
-      match a with
-      | Leaf => Node (set V Leaf ii v) None Leaf
-      | Node l o r => Node (set V l ii v) o r
-      end
-    | xI ii =>
-      match a with
-      | Leaf => Node Leaf None (set V Leaf ii v)
-      | Node l o r => Node l o (set V r ii v)
-      end
-    end.
+      | Leaf => None
+      | Node l o r =>
+          match key with
+          | xH => o
+          | xO ii => get l ii
+          | xI ii => get r ii
+          end
+      end.
+
+    Lemma get_empty:
+      forall (k: positive),
+        get empty k = None.
+    Proof.
+      induction k; auto.
+    Qed.
+  End GET.
+
+  Section SET.
+    Variable V: Type.
+
+    Fixpoint set (a: t V) (key: positive) (v: V): t V :=
+      match key with
+      | xH =>
+        match a with
+        | Leaf => Node Leaf (Some v) Leaf
+        | Node l _ r => Node l (Some v) r
+        end
+      | xO ii =>
+        match a with
+        | Leaf => Node (set Leaf ii v) None Leaf
+        | Node l o r => Node (set l ii v) o r
+        end
+      | xI ii =>
+        match a with
+        | Leaf => Node Leaf None (set Leaf ii v)
+        | Node l o r => Node l o (set r ii v)
+        end
+      end.
+
+    Lemma set_eq:
+      forall (t: t V) (k: key) (v: V),
+        get (set t k v) k = Some v.
+    Proof.
+      intros t k. generalize dependent t.
+      induction k; intros t v; destruct t; simpl; auto.
+    Qed.
+
+    Lemma set_ne:
+      forall (t: t V) (ks: key) (kg: key) (v: V),
+        ks <> kg -> 
+        get (set t ks v) kg = get t kg.
+    Proof.
+      intros t ks kg. generalize dependent ks. generalize dependent t.
+      induction kg; intros t ks v ne; destruct ks; destruct t; simpl;
+        try apply IHkg; simpl; congruence.
+    Qed.
+
+    Lemma set_get:
+      forall (t: t V) (ks: key) (kg: key) (v: V), 
+        get (set t ks v) kg = if Pos.eqb ks kg then Some v else get t kg.
+    Proof.
+      induction t0; intros ks kg v; destruct (Pos.eqb ks kg) eqn:E.
+      + rewrite Pos.eqb_eq in E. subst kg. apply set_eq.
+      + apply set_ne. intros contra. subst kg.
+        assert (Pos.eqb ks ks = true). apply Pos.eqb_eq. reflexivity.
+        rewrite E in H. inversion H.
+      + apply Pos.eqb_eq in E. subst kg.
+        apply set_eq.
+      + apply set_ne. intros contra. subst kg.
+        assert (Pos.eqb ks ks = true). apply Pos.eqb_eq. reflexivity.
+        rewrite E in H. inversion H.
+    Qed.
+  End SET.
 
   Fixpoint remove (V: Type) (a: t V) (key: positive): t V :=
     match a with
@@ -110,14 +162,14 @@ Module PTrie <: PARTIAL_MAP.
     | Node l o r =>
       match key with
       | xH => Node l None r
-      | xO ii => Node (remove V l ii) o r
-      | xI ii => Node l o (remove V r ii)
+      | xO ii => Node (remove l ii) o r
+      | xI ii => Node l o (remove r ii)
       end
     end.
 
   Fixpoint append (l: positive) (r: positive): positive :=
     match l with
-    | xH => l
+    | xH => r
     | xO i => xO (append i r)
     | xI i => xI (append i r)
     end.
@@ -145,7 +197,7 @@ Module PTrie <: PARTIAL_MAP.
 
     Theorem map_opt_correct:
       forall (t: t A) (k: key) (b: B),
-         Some b = get B (map_opt t) k -> exists a, (Some a = get A t k /\ Some b = f k a).
+         Some b = get (map_opt t) k -> exists a, (Some a = get t k /\ Some b = f k a).
     Admitted.
   End MAP_OPT.
 
@@ -153,11 +205,11 @@ Module PTrie <: PARTIAL_MAP.
     Variables A B: Type.
     Variable f: key -> A -> B.
 
-    Definition map (a: t A): t B := map_opt A B (fun k a => Some (f k a)) a.
+    Definition map (a: t A): t B := map_opt (fun k a => Some (f k a)) a.
 
     Theorem map_in :
       forall (t: t A) (k: key) (b: B),
-        Some b = get B (map t) k -> exists (a: A), Some a = get A t k /\ b = f k a.
+        Some b = get (map t) k -> exists (a: A), Some a = get t k /\ b = f k a.
     Proof.
       intros t k b.
       intros Hmapped.
@@ -169,67 +221,96 @@ Module PTrie <: PARTIAL_MAP.
 
     Theorem map_get :
       forall (t: t A) (k: key),
-        get B (map t) k = option_map (f k) (get A t k).
+        get (map t) k = option_map (f k) (get t k).
     Admitted.
   End MAP.
 
-  Fixpoint fold_helper (A: Type) (B: Type) (f: B -> key -> A -> B) (key: key) (t: t A) (v: B) : B :=
-    match t with
-    | Leaf => v
-    | Node l None r =>
-       let r' := fold_helper A B f (append key (xO xH)) r v in
-       fold_helper A B f (append key (xI xH)) l r'
-    | Node l (Some o) r =>
-       let r' := fold_helper A B f (append key (xO xH)) r v in
-       let o' := f r' key o in
-       fold_helper A B f (append key (xI xH)) l o'
-    end.
-
-  Fixpoint fold (A: Type) (B: Type) (f: B -> key -> A -> B) (t: t A) (v: B) :=
-    fold_helper A B f xH t v.
-
   Section TO_LIST.
     Variable V: Type.
-    Fixpoint to_list_helper (t: t V) (k: key) (acc: list (key * V)) :=
+    Fixpoint to_list_helper (k: key) (t: t V) (acc: list (key * V)) :=
       match t with
       | Leaf => acc
       | Node l None r =>
-        let r' := to_list_helper r (append (xI xH) k) acc in
-        to_list_helper r (append (xO xH) k) acc
+        let r' := to_list_helper (append k (xI xH)) r acc in
+        to_list_helper (append k (xO xH)) l r'
       | Node l (Some v) r =>
-        let r' := to_list_helper r (append (xI xH) k) acc in
+        let r' := to_list_helper (append k (xI xH)) r acc in
         let v' := (k, v) :: r' in
-        to_list_helper r (append (xO xH) k) acc
+        to_list_helper (append (xO xH) k) l v'
       end.
 
-    Definition to_list (t: t V) := to_list_helper t xH [].
+    Definition to_list (t: t V) := to_list_helper xH t [].
+
+    Lemma to_list_helper_correct:
+      forall (t: t V) (k: positive) (j: positive) (v: V) (acc: list (key * V)),
+        Some v = get t k -> In (append j k, v) (to_list_helper j t acc).
+    Admitted.
 
     Theorem to_list_correct:
       forall (t: t V) (k: key) (v: V),
-        In (k, v) (to_list t) -> Some v = get V t k.
-    Admitted.
+        Some v = get t k -> In (k, v) (to_list t).
+    Proof.
+      intros t k v Hin.
+      apply ((to_list_helper_correct t k xH) v [] Hin).
+    Qed.
   End TO_LIST.
+
+  Arguments to_list {V}.
+
+  Section FOLD.
+    Variable A: Type.
+    Variable B: Type.
+    Variable f: B -> key -> A -> B.
+
+    Fixpoint fold_helper (k: key) (t: t A) (v: B) : B :=
+      match t with
+      | Leaf => v
+      | Node l None r =>
+         let l' := fold_helper (append k (xO xH)) l v in
+         fold_helper (append k (xI xH)) r l'
+      | Node l (Some o) r =>
+         let l' := fold_helper (append k (xO xH)) l v in
+         let o' := f l' k o in
+         fold_helper (append k (xI xH)) r o'
+      end.
+
+    Fixpoint fold (t: t A) (v: B) :=
+      fold_helper xH t v.
+
+    Theorem fold_list:
+      forall (t: t A) (v: B),
+        fold t v = List.fold_left (fun a p => f a (fst p) (snd p)) (to_list t) v.
+    Admitted.
+
+    Theorem fold_prop:
+      forall 
+        (t: t A)
+        (pB: B -> Prop) 
+        (pE: key -> A -> Prop)
+        (pK: forall (k: key) (a: A) (acc: B), pB acc -> pE k a -> pB (f acc k a))
+        (b: B),
+        pB b -> pB (fold t b).
+    Admitted.
+
+  End FOLD.
 
   Section VALUES.
     Variable V: Type.
 
     Definition values (t: t V) := 
-      List.map (fun elem => match elem with (_, v) => v end) (to_list V t).
+      List.map (fun elem => match elem with (_, v) => v end) (to_list t).
 
     Theorem values_correct:
-      forall (t: t V) (v: V),
-        In v (values t) -> exists k, Some v = get V t k.
+      forall (t: t V) (k: key) (v: V),
+        Some v = get t k -> In v (values t).
     Proof.
-      intros t v.
+      intros t k v.
       intros Helem.
-      apply in_map_iff in Helem.
-      destruct Helem as [x H].
-      destruct x as [k].
-      exists k.
-      destruct H as [Heq Hin].
-      rewrite Heq in Hin.
-      apply to_list_correct in Hin.
-      apply Hin.
+      apply in_map_iff.
+      exists (k, v).
+      split. auto.
+      apply to_list_correct.
+      apply Helem.
     Qed.
   End VALUES.
 
@@ -237,20 +318,20 @@ Module PTrie <: PARTIAL_MAP.
     Variable V: Type.
 
     Definition extract (t: t (key * V)) :=
-      fold (key * V) (PTrie.t V)
+      fold
         (fun tree _ v =>
           match v with
-          | (k, v') => set V tree k v'
+          | (k, v') => set tree k v'
           end)
         t
-        (PTrie.empty V).
+        PTrie.empty.
 
     Theorem extract_correct:
       forall (e: t (key *  V)) (k: key) (v: V),
-        Some v = get V (extract e) k -> exists k', Some (k, v) = get (key * V) e k'.
+        Some v = get (extract e) k -> exists k', Some (k, v) = get e k'.
     Admitted.
   End EXTRACT.
-
+  
   Section COMBINE.
     Variables A B C: Type.
     Variable f: option A -> option B -> option C.
@@ -265,7 +346,7 @@ Module PTrie <: PARTIAL_MAP.
 
     Theorem combine_l_correct:
       forall (a: t A) (k: key),
-        get C (combine_l a) k = f (get A a k) None.
+        get (combine_l a) k = f (get a k) None.
     Proof.
       intros a.
       induction a; intros k; simpl.
@@ -283,7 +364,7 @@ Module PTrie <: PARTIAL_MAP.
 
     Theorem combine_r_correct:
       forall (b: t B) (k: key),
-        get C (combine_r b) k = f None (get B b k).
+        get (combine_r b) k = f None (get b k).
     Proof.
       intros a.
       induction a; intros k; simpl.
@@ -303,7 +384,7 @@ Module PTrie <: PARTIAL_MAP.
 
     Theorem combine_correct:
       forall (a: t A) (b: t B) (c: t C) (k: key),
-        get C (combine a b) k = f (get A a k) (get B b k).
+        get (combine a b) k = f (get a k) (get b k).
     Proof.
       intros a.
       induction a; intros b c k.
@@ -334,7 +415,7 @@ Module PTrie <: PARTIAL_MAP.
 
     Definition eq (t1: t V) (t2: t V) : Prop :=
       forall key,
-        match get V t1 key, get V t2 key with
+        match get t1 key, get t2 key with
         | None, None => True
         | Some v1, Some v2 => eqV v1 v2
         | _, _ => False
@@ -347,7 +428,7 @@ Module PTrie <: PARTIAL_MAP.
       intros t.
       unfold eq.
       intros key.
-      destruct (get V t key).
+      destruct (get t key).
       - apply eqV_refl.
       - reflexivity.
     Qed.
@@ -360,7 +441,7 @@ Module PTrie <: PARTIAL_MAP.
       unfold eq.
       intros H key.
       generalize (H key).
-      destruct (get V t1 key); destruct (get V t2 key); try auto.
+      destruct (get t1 key); destruct (get t2 key); try auto.
     Qed.
 
     Lemma eq_trans:
@@ -372,8 +453,8 @@ Module PTrie <: PARTIAL_MAP.
       intros key.
       generalize (H12 key).
       generalize (H23 key).
-      destruct (get V t1 key); destruct (get V t2 key); destruct (get V t3 key); try auto.
-      - intro H0. intro H1. apply (eqV_trans v v0 v1); auto.
+      destruct (get t1 key); destruct (get t2 key); destruct (get t3 key); try auto.
+      - intro H0. intro H1. apply eqV_trans with (v2 := v0); assumption.
       - intro H'. destruct H'.
     Qed.
   End EXTENSIONAL_EQUALITY.
@@ -395,7 +476,7 @@ Module PTrie <: PARTIAL_MAP.
 
     Theorem is_empty_correct:
       forall t,
-        is_empty t = true -> forall key, get V t key = None.
+        is_empty t = true -> forall key, get t key = None.
     Proof.
       intros t.
       intro H.
@@ -455,7 +536,8 @@ Module PTrie <: PARTIAL_MAP.
 
     Theorem eqb_correct:
       forall t1 t2,
-        eqb t1 t2 = true -> forall k, get V t1 k = get V t2 k.
+        eqb t1 t2 = true -> 
+        forall k, get t1 k = get t2 k.
     Admitted.
 
     Theorem eqb_node:
@@ -517,7 +599,7 @@ Module PTrie <: PARTIAL_MAP.
     Qed.
 
     Theorem eqb_eq:
-      forall t1 t2, eqb t1 t2 = true -> eq V eqV t1 t2.
+      forall t1 t2, eqb t1 t2 = true -> eq eqV t1 t2.
     Proof.
       induction t1.
       {
@@ -535,9 +617,9 @@ Module PTrie <: PARTIAL_MAP.
           rewrite Ho.
           rewrite andb_true_iff in H1.
           destruct H1 as [Ht1 Ht2].
-          assert (Hh1: forall key, get V t0_1 key = None).
+          assert (Hh1: forall key, get t0_1 key = None).
           {  intro k'. apply is_empty_correct. apply Ht1. }
-          assert (Hh2: forall key, get V t0_2 key = None).
+          assert (Hh2: forall key, get t0_2 key = None).
           {  intro k'. apply is_empty_correct. apply Ht2. }
           destruct k; try (rewrite Hh2); try (rewrite Hh1); reflexivity.
       }
@@ -554,9 +636,9 @@ Module PTrie <: PARTIAL_MAP.
           rewrite Ho.
           rewrite andb_true_iff in H1.
           destruct H1 as [Ht1 Ht2].
-          assert (Hh1: forall key, get V t1_1 key = None).
+          assert (Hh1: forall key, get t1_1 key = None).
           {  intro k'. apply is_empty_correct. apply Ht1. }
-          assert (Hh2: forall key, get V t1_2 key = None).
+          assert (Hh2: forall key, get t1_2 key = None).
           {  intro k'. apply is_empty_correct. apply Ht2. }
           destruct k; try (rewrite Hh2); try (rewrite Hh1); reflexivity.
         }
@@ -568,12 +650,12 @@ Module PTrie <: PARTIAL_MAP.
           apply IHt1_1 in Hl. unfold eq in Hl.
           apply IHt1_2 in Hr. unfold eq in Hr.
           destruct k; simpl.
-          - destruct (get V t1_2 k) eqn:E1; destruct (get V t0_2 k) eqn:E2;
+          - destruct (get t1_2 k) eqn:E1; destruct (get t0_2 k) eqn:E2;
               generalize (Hr k); intros Hgetr; rewrite E1 in Hgetr; rewrite E2 in Hgetr;
               try inversion Hgetr.
             + apply Hgetr.
             + reflexivity.
-          - destruct (get V t1_1 k) eqn:E1; destruct (get V t0_1 k) eqn:E2;
+          - destruct (get t1_1 k) eqn:E1; destruct (get t0_1 k) eqn:E2;
               generalize (Hl k); intros Hgetl; rewrite E1 in Hgetl; rewrite E2 in Hgetl;
               try inversion Hgetl.
             + apply Hgetl.
@@ -593,7 +675,7 @@ Module PTrie <: PARTIAL_MAP.
     Qed.
   End BOOLEAN_EQUALITY.
 
-  Section DECIDABILITY.
+  Section ELEMENT.
     Variable V: Type.
 
     Hypothesis eq_decV: 
@@ -625,11 +707,18 @@ Module PTrie <: PARTIAL_MAP.
           right. unfold not. intros H.
           destruct H; auto.
     Qed.
-  End DECIDABILITY.
+  End ELEMENT.
+
+  Arguments Elem {V}.
 End PTrie.
 
-
-Arguments PTrie.get {V}.
-Arguments PTrie.eqb {V}.
-
 Notation "a ! b" := (PTrie.get a b) (at level 1).
+
+Notation "{ }" := PTrie.empty.
+Notation "{ k ! v }" := (PTrie.set PTrie.empty k v).
+
+Notation "{ e0 ; e1 ; .. ; en }" :=
+  (PTrie.set 
+    (PTrie.set .. (PTrie.set PTrie.empty (fst en) (snd en)) .. 
+     (fst e1) (snd e1)) 
+   (fst e0) (snd e0)).
