Closure.v
@@ -1,0 +1,219 @@
+(* This file is part of the LLIR Semantics project. *)
+(* Licensing information is available in the LICENSE file. *)
+(* (C) 2020 Nandor Licker. All rights reserved. *)
+
+Require Import Coq.ZArith.ZArith.
+Require Import Coq.Lists.List.
+Require Import Coq.funind.FunInd.
+Require Import Coq.funind.Recdef.
+
+Require Import LLIR.Maps.
+Require Import LLIR.State.
+
+Import ListNotations.
+
+
+
+Definition relation := PTrie.t reg.
+
+
+Section CLOSURE.
+
+  Variable loads: relation.
+
+  Inductive chain: reg -> reg -> Prop :=
+    | closure_chain_elem:
+      forall (dst: reg) (src: reg)
+        (HE: Some src = loads ! dst),
+        chain dst src
+    | closure_chain_step:
+      forall (dst: reg) (mid: reg) (src: reg)
+        (HL: chain mid src)
+        (HR: chain dst mid),
+        chain dst src
+    .
+
+  Definition is_relation (l: relation): Prop :=
+    forall (dst: reg) (src: reg),
+      Some src = l ! dst -> chain dst src.
+
+  Lemma is_valid_empty: 
+    is_relation PTrie.empty.
+  Proof. 
+    intros dst src Hin. inversion Hin.
+  Qed.
+
+  Hypothesis H_loads_valid: is_relation loads.
+
+  Definition find_match (l: relation) (src: reg): reg :=
+    match l ! src with
+    | None => src
+    | Some dst => dst
+    end.
+
+  Lemma find_match_chain:
+    forall (l: relation),
+      is_relation l -> 
+      forall (s: reg) (s': reg),
+        s' = find_match l s -> s = s' \/ chain s s'.
+  Proof.
+    intros l Hvalid src src' Hfind.
+    unfold find_match in Hfind.
+    destruct (l ! src) eqn:E; try symmetry in E.
+    - right. apply Hvalid. subst src'. auto.
+    - left. auto.
+  Qed.
+
+  Definition update_map (l: relation) (d': reg) (s': reg): relation :=
+    PTrie.map (fun d s => if Pos.eqb s d' then s' else s) l.
+
+  Example update_map_example :=
+    { (2%positive, 3%positive)
+    ; (1%positive, 3%positive)
+    ; (5%positive, 3%positive)
+    }.
+
+  Example update_map_example' := 
+    update_map update_map_example 3%positive 5%positive.
+
+  Fact update_map_2: update_map_example' ! 2%positive = Some 5%positive.
+  Proof. auto. Qed.
+  Fact update_map_1: update_map_example' ! 1%positive = Some 5%positive.
+  Proof. auto. Qed.
+  Fact update_map_5: update_map_example' ! 5%positive = Some 5%positive.
+  Proof. auto. Qed.
+
+  Lemma update_map_chain:
+    forall (l: relation),
+      is_relation l ->
+      forall (d: reg) (s: reg),
+        chain d s ->
+        is_relation (update_map l d s).
+  Proof.
+    intros l Hvalid d s Hin d' s' Hdef.
+    unfold update_map in Hdef.
+    apply PTrie.map_in in Hdef.
+    destruct Hdef as [a [Heq Hif]].
+    destruct (Pos.eqb a d) eqn:E.
+    - apply Pos.eqb_eq in E. subst a s'.
+      apply (closure_chain_step d' d s).
+      apply Hin.
+      apply Hvalid. apply Heq.
+    - subst. apply Hvalid. apply Heq.
+  Qed.
+
+  Definition closure_helper (acc: relation) (dst: reg) (src: reg): relation :=
+    let src' := find_match acc src in
+    let acc_u := update_map acc dst src' in
+    PTrie.set acc_u dst src'.
+
+  Definition closure_helper_valid:
+    forall (dst: PTrie.key) (src: reg) (acc: relation),
+      is_relation acc ->
+      Some src = loads ! dst ->
+      is_relation (closure_helper acc dst src).
+  Proof.
+    intros dst src acc Hvalid_acc Helem dst' src' Helem'.
+    unfold closure_helper in Helem'.
+    remember (find_match acc src) as s'.
+    remember (update_map acc dst s') as acc'.
+    rewrite PTrie.set_get in Helem'.
+    destruct (Pos.eqb dst dst') eqn:E.
+    {
+      apply Pos.eqb_eq in E. subst dst.
+      inversion Helem'. subst s'.
+      generalize (find_match_chain acc Hvalid_acc src src' H0).
+      intros Hfm.
+      rewrite <- H0.
+      destruct Hfm.
+      {
+        subst src.
+        apply H_loads_valid.
+        apply Helem.
+      }
+      {
+        apply closure_chain_step with (mid := src). 
+        apply H.
+        apply H_loads_valid. apply Helem.
+      }
+    }
+    {
+      assert (Hchain: chain dst s').
+      {
+        generalize (find_match_chain acc Hvalid_acc src s' Heqs').
+        intros Hfm.
+        destruct Hfm.
+        {
+          subst src.
+          apply H_loads_valid. apply Helem.
+        }
+        {
+          apply closure_chain_step with (mid := src).
+          apply H.
+          apply H_loads_valid. apply Helem.
+        }
+      }
+      assert (Hvalid_acc': is_relation acc').
+      {
+        generalize (update_map_chain acc Hvalid_acc dst s' Hchain).
+        intros Hvalid.
+        subst acc'.
+        apply Hvalid.
+      }
+      apply Hvalid_acc'.
+      apply Helem'.
+    }
+  Qed.
+
+  Example closure_helper_example :=
+    { (2%positive, 5%positive)
+    ; (3%positive, 5%positive)
+    }.
+
+  Definition closure_helper_example' :=
+    closure_helper closure_helper_example 5%positive 6%positive.
+
+  Fact closure_helper_2: closure_helper_example' ! 2%positive = Some 6%positive.
+  Proof. auto. Qed.
+  Fact closure_helper_3: closure_helper_example' ! 3%positive = Some 6%positive.
+  Proof. auto. Qed.
+  Fact closure_helper_5: closure_helper_example' ! 5%positive = Some 6%positive.
+  Proof. auto. Qed.
+
+  Definition closure (l: relation) :=
+    PTrie.fold closure_helper l PTrie.empty.
+
+  Definition closure_valid:
+    is_relation (closure loads).
+  Proof.
+    unfold closure.
+    apply (PTrie.fold_prop 
+      closure_helper 
+      loads
+      is_relation
+      (fun k v => Some v = loads ! k)
+      closure_helper_valid
+      {}
+      is_valid_empty
+    ).
+  Qed.
+
+  Example chain_example :=
+    { ( 4%positive, 3%positive)
+    ; ( 3%positive, 2%positive)
+    ; ( 2%positive, 1%positive)
+    }.
+
+  Definition chain_example' := closure chain_example.
+
+  Fact chain_4: chain_example' ! 4%positive = Some 1%positive.
+  Proof. auto. Qed.
+  Fact chain_3: chain_example' ! 3%positive = Some 1%positive.
+  Proof. auto. Qed.
+  Fact chain_2: chain_example' ! 2%positive = Some 1%positive.
+  Proof. auto. Qed.
+
+End CLOSURE.
+
+
+
