StoreToLoad.v
@@ -8,6 +8,7 @@ Require Import Coq.Lists.List.
 Require Import LLIR.Aliasing.
 Require Import LLIR.LLIR.
 Require Import LLIR.Maps.
+Require Import LLIR.Closure.
 Require Import LLIR.State.
 Require Import LLIR.Values.
 Require Import LLIR.Verify.
@@ -20,7 +21,7 @@ Import ListNotations.
 
 
 Definition find_load_reg (insts: inst_map) (rs: reaching_stores) (aa: points_to_set): PTrie.t reg :=
-  PTrie.extract reg (PTrie.map_opt inst (reg * reg) 
+  PTrie.extract (PTrie.map_opt 
     (fun k inst =>
       match inst with
       | LLLd addr dst next =>
@@ -42,19 +43,17 @@ Definition rewrite_reg (loads: PTrie.t reg) (r: reg): reg :=
   | Some reg' => reg'
   end.
 
-
 Definition rewrite_inst (i: inst) (loads: PTrie.t reg): inst :=
   rewrite_uses i (rewrite_reg loads).
 
-
 Definition rewrite_insts (insts: inst_map) (loads: PTrie.t reg): inst_map :=
-  PTrie.map inst inst (fun k inst => rewrite_inst inst loads) insts.
+  PTrie.map (fun k inst => rewrite_inst inst loads) insts.
 
 
 Definition propagate_store_to_load (f: func): func :=
   let aa := local_pta f in
   let rs := analyse_reaching_stores f aa in
-  let loads := find_load_reg f.(fn_insts) rs aa in
+  let loads := closure (find_load_reg f.(fn_insts) rs aa) in
   let fn_insts := rewrite_insts f.(fn_insts) loads in
   mkfunc f.(fn_args) f.(fn_stack) fn_insts f.(fn_phis) f.(fn_entry).
 
@@ -63,21 +62,32 @@ Section LOAD_PROPERTIES.
   Variable f: func.
   Variable rs: reaching_stores.
   Variable aa: points_to_set.
+  Variable loads: relation.
+  Variable loads': relation.
 
   Hypothesis H_f_valid: is_valid f.
+  Hypothesis Heqloads: loads = find_load_reg f.(fn_insts) rs aa.
+  Hypothesis Heqloads': loads' = closure loads.
+
+  Lemma H_loads_relation: is_relation loads loads.
+  Proof. 
+    intros dst src. intros H. apply closure_chain_elem. apply H.
+  Qed.
+
+  Lemma H_loads_relation': is_relation loads loads'.
+  Proof.
+    subst loads'. apply closure_valid. apply H_loads_relation.
+  Qed.
 
   Lemma propagate_src_dst:
-    forall (loads: PTrie.t reg) (dst: reg) (src: reg),
-      loads = find_load_reg f.(fn_insts) rs aa ->
+    forall (dst: reg) (src: reg),
       Some src = PTrie.get loads dst ->
         exists (k: node) (addr: reg) (object: positive) (offset: positive),
           loads_from f aa k dst addr object offset /\
           store_reaches rs k src object offset.
   Proof.
-    intros loads src dst.
-    intro Hprop.
-    intro Helem.
-    rewrite Hprop in Helem.
+    intros src dst Helem.
+    subst loads.
     apply PTrie.extract_correct in Helem.
     destruct Helem as [k Helem].
     exists k.
@@ -88,173 +98,30 @@ Section LOAD_PROPERTIES.
     destruct (get_load_addr aa addr) eqn:Hload; inversion Hfunc; clear H0.
     destruct (get_store_to rs k o) eqn:Hstore; inversion Hfunc; clear H0.
     destruct o as [object offset].
-    exists addr.
-    exists object.
-    exists offset.
+    exists addr. exists object. exists offset.
     inversion Hfunc.
-    rewrite <- H0 in Hfunc. 
-    rewrite <- H0. 
-    rewrite <- H0 in Hinst. 
-    rewrite <- H2. 
+    rewrite <- H0 in *.
     rewrite <- H2 in Hstore.
     split.
     - apply load with (next := next). symmetry. apply Hload. apply Hinst.
-    - apply store. symmetry. apply Hstore.
+    - apply store. symmetry. subst. apply Hstore.
   Qed.
 
-  Definition reg_dom (src: reg) (dst: reg): Prop :=
-    forall (def: node) (use: node),
-      DefinedAt f def src ->
-      UsedAt f use dst ->
-      StrictlyDominates f def use.
+  Lemma propagate_src_dst_chain:
+    forall (dst: reg) (src: reg),
+      chain loads dst src ->
+        exists (k: node) (addr: reg) (object: positive) (offset: positive),
+          loads_from f aa k dst addr object offset /\
+          store_reaches rs k src object offset.
+  Admitted.
 
-  Lemma src_dominates_dst:
-    forall (loads: PTrie.t reg) (src: reg) (dst: reg),
-      loads = find_load_reg f.(fn_insts) rs aa ->
-      Some src = PTrie.get loads dst -> 
-      reg_dom src dst.
-  Proof.
-    intros loads src dst.
-    intro Hprop.
-    intro Helem.
-    apply (propagate_src_dst loads dst src Hprop) in Helem.
-    destruct Helem as [k Helem].
-    destruct Helem as [ld_addr Helem].
-    destruct Helem as [object Helem].
-    destruct Helem as [offset Helem].
-    destruct Helem as [Hload Hstore].
-    assert (Hstore': store_reaches rs k src object offset).
-    { apply Hstore. }
-    apply (reaching_store_origin f aa) in Hstore'.
-    destruct Hstore' as [store Hstore'].
-    destruct Hstore' as [val Hstore'].
-    destruct Hstore' as [next Hstore'].
-    destruct Hstore' as [Hstore' Hdom].
-    inversion Hstore'.
-    assert (H_f_valid': is_valid f). { apply H_f_valid. }
-    destruct H_f_valid' as [Hdef_dom_uses Hdefs_unique _].
-    unfold defs_are_unique in Hdefs_unique.
-    intros def use.
-    intros Hdef_src.
-    intros Huse_dst.
-    apply (sdom_trans f def store use).
-    {
-      generalize (Hdef_dom_uses store).
-      intros H'.
-      assert (Hsrc_used_at_store: UsedAt f store src).
-      { unfold UsedAt. rewrite <- H. unfold Uses. auto. }
-      destruct ((fn_insts f) ! def) eqn:E.
-      {
-        symmetry in E.
-        generalize (H' src Hsrc_used_at_store).
-        intros H''.
-        destruct H'' as [def' [Hdef' Hdom']].
-        assert (def = def').
-        { apply Hdefs_unique with (r := src). apply Hdef'. apply Hdef_src. }
-        subst.
-        apply Hdom'.
-      }
-      {
-        unfold DefinedAt in Hdef_src.
-        rewrite E in Hdef_src.
-        inversion Hdef_src.
-      }
-    }
-    {
-      apply (sdom_trans f store k use).
-      {
-        inversion Hstore.
-        inversion Hstore'.
-        unfold get_store_to in H5.
-        destruct (rs ! k) as [use'|] eqn:Euse'; inversion H5.
-        destruct (use' ! object) as [object'|] eqn:Eobject'; inversion H5.
-        destruct (object' ! offset) as [offset'|] eqn:Eoffset'; inversion H5.
-        inversion H5. rewrite <- H5 in Eoffset'.
-        apply (reaching_stores_dom f aa rs k use' object object' offset src); 
-          try symmetry.
-        - apply Euse'.
-        - apply Eobject'.
-        - apply Eoffset'.
-        - apply (store_at f aa store object offset src addr0 next1).
-          + apply H10.
-          + apply H11.
-      }
-      {
-        inversion Hload.
-        unfold uses_have_defs in Hdef_dom_uses.
-        subst.
-        assert (HdefK: DefinedAt f k dst). 
-        { unfold DefinedAt. rewrite <- H6. unfold Defs. reflexivity. }
-        destruct (f.(fn_insts) ! use) eqn:Euse.
-        + generalize (Hdef_dom_uses use dst Huse_dst).
-          intros H''.
-          destruct H'' as [def' [Hdef' Hdom']].
-          assert (def' = k).
-          { apply Hdefs_unique with (r := dst).  apply HdefK. apply Hdef'. }
-          subst.
-          apply Hdom'.
-        + unfold UsedAt in Huse_dst.
-          rewrite Euse in Huse_dst.
-          inversion Huse_dst.
-      }
-    }
-  Qed.
-
-  Lemma propagate_load_unique:
-    forall (loads: PTrie.t reg) (dst: reg) (src: reg),
-      loads = find_load_reg f.(fn_insts) rs aa ->
-      Some src = PTrie.get loads dst ->
-        forall (src': reg), Some src' = PTrie.get loads dst -> src = src'.
-  Proof.
-    intros loads  dst src.
-    intro Hloads.
-    intro Hin.
-    intro src'.
-    intro Hin'.
-    generalize (propagate_src_dst loads dst src Hloads Hin).
-    intros Hexists.
-    generalize (propagate_src_dst loads dst src' Hloads Hin').
-    intros Hexists'.
-    destruct Hexists as [k [addr [object [offset [Hload Hstore]]]]].
-    destruct Hexists' as [k' [addr' [object' [offset' [Hload' Hstore']]]]].
-    inversion Hload.
-    assert (Hdef: Defs (LLLd addr dst next) dst). reflexivity.
-    destruct H_f_valid as [_ Hunique _].
-    unfold defs_are_unique in Hunique.
-    inversion Hload'.
-    generalize (Hunique k' k dst). intro Huniq.
-    assert (Hkk: k = k').
-    { 
-      apply Huniq; unfold DefinedAt.
-      - rewrite <- H7. unfold Defs. auto.
-      - rewrite <- H0. unfold Defs. auto.
-    }
-    assert (Hld_eq: LLLd addr dst next = LLLd addr' dst next0).
-    { subst. rewrite <- H0 in H7. inversion H7. trivial. }
-    inversion Hld_eq as [Haddr].
-    rewrite <- Haddr in H6.
-    rewrite <- H6 in H.
-    inversion H.
-    rewrite <- H15 in Hstore'.
-    rewrite <- H16 in Hstore'.
-    inversion Hstore.
-    inversion Hstore'.
-    subst.
-    rewrite <- H14 in H21.
-    inversion H21.
-    reflexivity.
-  Qed.
-
-  Lemma propagate_load_no_refl:
-    forall (loads: PTrie.t reg) (dst: reg) (src: reg),
-      loads = find_load_reg f.(fn_insts) rs aa ->
-      Some src = PTrie.get loads dst -> 
+  Lemma propagate_load_irrefl:
+    forall (dst: reg) (src: reg),
+      chain loads dst src -> 
       src <> dst.
   Proof.
-    intros loads dst src.
-    intros Hloads.
-    intros Hin.
-    apply propagate_src_dst in Hin; try apply Hloads.
+    intros dst src Hin.
+    apply propagate_src_dst_chain in Hin; try apply Hloads.
     intro contra. subst.
     destruct Hin as [k [addr [object [offset [Hload Hstore]]]]].
     inversion Hload.
@@ -287,75 +154,17 @@ Section LOAD_PROPERTIES.
     intros eq. apply STRICT in eq. inversion eq.
   Qed.
 
-  Lemma propagate_use_origin:
-    forall (loads: PTrie.t reg) (user: inst) (user': inst) (r: reg),
-      loads = find_load_reg f.(fn_insts) rs aa ->
-      user' = rewrite_inst user loads ->
-      Uses user r ->
-      (
-        (PTrie.get loads r = None /\ Uses user' r)
-        \/
-        (exists (r': reg), Some r' = PTrie.get loads r /\ Uses user' r')
-      ).
-  Proof.
-    intros loads user user' r Hloads Huser' Huses.
-    unfold rewrite_inst in Huser'.
-    unfold rewrite_uses in Huser'.
-    unfold rewrite_reg in Huser'.
-    destruct (PTrie.get loads r) eqn:Eload.
-    {
-      right.
-      exists r0.
-      split; auto.
-      destruct user; inversion Huses;
-        subst;
-        try rewrite Eload;
-        unfold Uses;
-        try reflexivity.
-      + left. reflexivity.
-      + right. reflexivity.
-      + left. reflexivity.
-      + unfold Uses in Huses.
-        destruct Huses.
-        - left. subst. rewrite Eload. reflexivity.
-        - right.
-          apply in_map_iff.
-          exists r.
-          split.
-          rewrite Eload. reflexivity.
-          apply H.
-      + left. reflexivity.
-      + right. reflexivity.
-    }
-    {
-      left.
-      split; try reflexivity.
-      destruct user; destruct Huses;
-        unfold Uses;
-        rewrite Huser';
-        try rewrite H;
-        try rewrite Eload;
-        auto.
-      right.
-      apply in_map_iff.
-      exists r.
-      rewrite Eload.
-      split. reflexivity. apply H.
-    }
-  Qed.
-
   Lemma propagate_use_inversion:
-    forall (loads: PTrie.t reg) (user: inst) (user': inst) (r: reg),
-      loads = find_load_reg f.(fn_insts) rs aa ->
-      user' = rewrite_inst user loads ->
+    forall (user: inst) (user': inst) (r: reg),
+      user' = rewrite_inst user loads' ->
       Uses user' r ->
       (
-        (PTrie.get loads r = None /\ Uses user r)
+        (PTrie.get loads' r = None /\ Uses user r)
         \/
-        (exists (r': reg), PTrie.get loads r' = Some r /\ Uses user r')
+        (exists (r': reg), PTrie.get loads' r' = Some r /\ Uses user r')
       ).
   Proof.
-    intros loads user user' r Hloads Huser' Huses.
+    intros user user' r Huser' Huses.
     rewrite Huser' in Huses.
     unfold rewrite_inst in Huses.
     unfold rewrite_uses in Huses.
@@ -367,51 +176,59 @@ Section LOAD_PROPERTIES.
     unfold Uses.
     destruct user eqn:Euser; destruct Huses;
       repeat match goal with
-      | [ |- context [loads ! ?reg] ] => 
-        destruct (loads ! reg) eqn:?reg
+      | [ |- context [loads' ! ?reg] ] => 
+        destruct (loads' ! reg) eqn:?reg
       | [ H: _ ! ?reg = Some ?v |- context [ _ ! _ = Some ?v ] ] => 
         right; exists reg; auto
       | [ H: _ = ?r |- context [ Some ?r ] ] => 
         rewrite <- H
       | [ H0: ?loads ! ?reg = None, H1: ?loads ! ?reg = Some _ |- _ ] =>
         rewrite H0 in H1; inversion H1
+      | [ H: ?a = ?b |- _ ] =>
+        subst b
       | [ |- _ ] =>
-        subst; auto
+        auto
       end.
     - right.
       apply in_map_iff in H.
       destruct H as [x [Hr Hin]].
-      remember (find_load_reg (fn_insts f) rs aa) as loads.
       destruct (Pos.eq_dec r x).
-      { 
-        destruct (loads ! x) eqn:E.
-        { 
-          generalize (propagate_load_no_refl loads x x).
-          intros Hrefl. 
-          apply Hrefl in Heqloads.
-          - contradiction Heqloads. reflexivity.
-          - symmetry. subst. apply E.
+      {
+        destruct (loads' ! x) eqn:E.
+        {
+          generalize (propagate_load_irrefl).
+          intros Hrefl.
+          subst r.
+          subst p0.
+          rewrite E in r0.
+          inversion r0.
+          subst p.
+          symmetry in E.
+          assert (Hchain: chain loads x x).
+          { apply H_loads_relation'. apply E. }
+          apply Hrefl in Hchain.
+          contradiction Hchain. auto.
         }
         {
           subst. rewrite E in r0. inversion r0.
         }
       }
       { 
-        destruct (loads ! x) eqn:E; subst.
+        destruct (loads' ! x) eqn:E; subst.
         * exists x. split. apply E. right. apply Hin.
         * rewrite E in r0. inversion r0.
       }
     - apply in_map_iff in H.
       destruct H as [x [Hr Hin]].
-      remember (find_load_reg (fn_insts f) rs aa) as loads.
       destruct (Pos.eq_dec r x).
       {
         left. rewrite e. auto.
       }
       {
-        destruct (loads ! x) eqn:E.
+        destruct (loads' ! x) eqn:E.
         {
-          subst. right. exists x. 
+          subst p.
+          right. exists x.
           split. apply E. right. apply Hin.
         }
         {
@@ -535,6 +352,7 @@ Section PROPAGATE_PROPERTIES.
     remember (local_pta f) as aa.
     remember (analyse_reaching_stores f aa) as rs.
     remember ((find_load_reg (fn_insts f) rs aa)) as loads.
+    remember (closure loads) as loads'.
     destruct H_f_valid as [Hdefs Huniq Hord].
     repeat split.
     (* Defs have uses *)
@@ -547,16 +365,21 @@ Section PROPAGATE_PROPERTIES.
       rewrite <- Heqaa in Hused.
       rewrite <- Heqrs in Hused.
       rewrite <- Heqloads in Hused.
+      rewrite <- Heqloads' in Hused.
       unfold UsedAt in Hused.
       simpl in Hused.
-      destruct ((rewrite_insts (fn_insts f) loads) ! use) as [user'|] eqn:E;
+      destruct ((rewrite_insts (fn_insts f) loads') ! use) as [user'|] eqn:E;
         try inversion Hused.
       unfold rewrite_insts in E.
       symmetry in E.
       apply PTrie.map_in in E.
       destruct E.
       destruct H as [Hin Hwr].
-      generalize (propagate_use_inversion f rs aa H_f_valid loads x user' r Heqloads Hwr Hused).
+      generalize (propagate_use_inversion 
+        f rs aa loads loads' 
+        H_f_valid Heqloads Heqloads'
+        x user' r
+        Hwr Hused).
       intros Hinv.
       generalize (Hdefs use r).
       intros Huse_implies_def.
@@ -607,8 +430,17 @@ Section PROPAGATE_PROPERTIES.
       }
       {
         destruct H as [r' [Hsubst Huse]].
-        symmetry in Hsubst.
-        generalize (propagate_src_dst f rs aa loads r' r Heqloads Hsubst).
+        assert (Hchain: chain loads r' r).
+        { 
+          apply (H_loads_relation' loads loads' Heqloads').
+          symmetry. apply Hsubst.
+        }
+        generalize (propagate_src_dst_chain
+          f rs aa loads loads' 
+          H_f_valid
+          Heqloads Heqloads' 
+          r' r
+          Hchain).
         intro Hprop.
         destruct Hprop as [k [addr [object [offset]]]].
         destruct H as [Hload Hstore].
